SemanticsUtil.dfy
@@ -8,10 +8,32 @@ module SemanticsUtil {
   import opened BoogieCfg
   import opened Wrappers
 
-  lemma WpShallowIfEquiv<A(!new)>(a: absval_interp<A>, guard: Expr, thn: Cmd, els: Cmd, post: WpPostShallow)
+
+  lemma WpShallowAssumeFalse<A(!new)>(a: absval_interp<A>, e: Expr, thn: Cmd, els: Cmd, post: Predicate<A>, s: state<A>)
+  requires ExprEvalBoolOpt(a, e, s) == Some(false)
+  ensures WpShallowSimpleCmd(a, Assume(e), post)(s) == Some(true)
+  { 
+  }
+
+  lemma WpShallowIfEquiv<A(!new)>(a: absval_interp<A>, guard: Expr, thn: Cmd, els: Cmd, post: WpPostShallow<A>, s: state<A>)
   requires LabelsWellDefAux(thn, post.scopes.Keys) && LabelsWellDefAux(els, post.scopes.Keys)
-  ensures WpShallow(a, If(Some(guard), thn, els), post) ==
-          WpShallow(a, If(None, Seq(SimpleCmd(Assume(guard)), thn), Seq(SimpleCmd(Assume(UnOp(Not, guard))), els)), post)
+  ensures WpShallow(a, If(Some(guard), thn, els), post)(s) ==
+          WpShallow(a, If(None, Seq(SimpleCmd(Assume(guard)), thn), Seq(SimpleCmd(Assume(UnOp(Not, guard))), els)), post)(s)
+  {  
+    calc {
+      WpShallow(a, If(Some(guard), thn, els), post)(s);
+      { WpShallowIfEquiv2(a, guard, thn, els, post, s); }
+      Util.AndOpt(
+        WpShallowSimpleCmd(a, Assume(guard), WpShallow(a, thn, post))(s),
+        WpShallowSimpleCmd(a, Assume(UnOp(Not, guard)), WpShallow(a, els, post))(s)
+      );
+      Util.AndOpt(
+        WpShallow(a, Seq(SimpleCmd(Assume(guard)), thn), post)(s),
+        WpShallow(a, Seq(SimpleCmd(Assume(UnOp(Not, guard))), els), post)(s)
+      );
+      WpShallow(a, If(None, Seq(SimpleCmd(Assume(guard)), thn), Seq(SimpleCmd(Assume(UnOp(Not, guard))), els)), post)(s);
+    }
+  }
 
   lemma WpShallowIfEquiv2<A(!new)>(a: absval_interp<A>, guard: Expr, thn: Cmd, els: Cmd, post: WpPostShallow, s: state<A>)
   requires LabelsWellDefAux(thn, post.scopes.Keys) && LabelsWellDefAux(els, post.scopes.Keys)
@@ -20,13 +42,113 @@ module SemanticsUtil {
             WpShallowSimpleCmd(a, Assume(guard), WpShallow(a, thn, post))(s),
             WpShallowSimpleCmd(a, Assume(UnOp(Not, guard)), WpShallow(a, els, post))(s)
           )
-  
+          //TODO maybe use proof from above and then apply this lemma for above proof
+  {
+    var guardOptVal := ExprEvalBoolOpt(a, guard, s);
+
+    if(guardOptVal.Some?) {
+      var guardVal := guardOptVal.value;
+
+      var actualAssume := if guardVal then Assume(guard) else Assume(UnOp(Not, guard));
+      var actualBranch := if guardVal then thn else els;
+
+      var trivialAssume := if !guardVal then Assume(guard) else Assume(UnOp(Not, guard));
+      var trivialBranch := if !guardVal then thn else els;
+
+      calc {
+        WpShallow(a, If(Some(guard), thn, els), post)(s);
+        WpShallow(a, actualBranch, post)(s);
+        WpShallowSimpleCmd(a, actualAssume, WpShallow(a, actualBranch, post))(s);
+      }
+
+      calc {
+        WpShallow(a, Seq(SimpleCmd(trivialAssume), trivialBranch), post)(s);
+        WpShallowSimpleCmd(a, trivialAssume, WpShallow(a, trivialBranch, post))(s);
+        Some(true);
+      }
+    } else {
+      calc {
+        WpShallowSimpleCmd(a, Assume(guard), WpShallow(a, thn, post))(s);
+        None;
+      }
+
+      calc {
+        Util.AndOpt(WpShallow(a, Seq(SimpleCmd(Assume(guard)), thn), post)(s), WpShallow(a, Seq(SimpleCmd(Assume(UnOp(Not, guard))), els), post)(s));
+        None;
+        WpShallow(a, If(Some(guard), thn, els), post)(s);
+      }
+    }
+  } 
+
+  lemma WpCfgConjunctionIndepOutsideCover<A(!new)>(a: absval_interp<A>, cfg: Cfg, updatedBlock: (BlockId, SimpleCmd), entries: seq<BlockId>, p: Predicate<A>, cover: set<BlockId>)
+    requires |entries| > 0
+    requires cfg.successors.Keys <= cfg.blocks.Keys
+    requires updatedBlock.0 !in cover
+    requires updatedBlock.0 in cfg.successors.Keys
+    ensures 
+      var cfg' := Cfg(cfg.entry, cfg.blocks[updatedBlock.0 := updatedBlock.1], cfg.successors);
+      WpCfgConjunction(a, cfg, entries, p, cover) == WpCfgConjunction(a, cfg', entries, p, cover);
+    decreases cover, 1, entries
+  {
+    WpCfgIndepOutsideCover(a, cfg, updatedBlock, entries[0], p, cover);
+  }
+
+  lemma WpCfgIndepOutsideCover<A(!new)>(a: absval_interp<A>, cfg: Cfg, updatedBlock: (BlockId, SimpleCmd), entry: BlockId, p: Predicate<A>, cover: set<BlockId>)
+    requires cfg.successors.Keys <= cfg.blocks.Keys
+    requires updatedBlock.0 !in cover
+    requires updatedBlock.0 in cfg.successors.Keys
+    ensures 
+      var cfg' := Cfg(cfg.entry, cfg.blocks[updatedBlock.0 := updatedBlock.1], cfg.successors);
+      WpCfg(a, cfg, entry, p, cover) == WpCfg(a, cfg', entry, p, cover);
+  decreases cover, 0
+  {
+    var (updId, updCmd) := updatedBlock;
+    var cfg' := Cfg(cfg.entry, cfg.blocks[updId := updCmd], cfg.successors);
+
+    if IsAcyclic(cfg.successors, entry, cover) {
+      var successors := if entry in cfg.successors.Keys then cfg.successors[entry] else [];
+      if successors != [] {
+        assert updId != entry; //since entry is in cover, but updId is not
+        WpCfgConjunctionIndepOutsideCover(a, cfg, updatedBlock, successors, p, cover-{entry});
+      } else {
+        /* If entry in cfg.successors.Keys, then we get that updId != entry for the same
+        reason as in the above branch. Otherwise, we get that updId != entry because
+        updId in cfg.successors.Keys. */
+      }
+    }
+  }
+
   lemma WpCfgEntrySplit<A(!new)>(a: absval_interp<A>, cfg: Cfg, entry: BlockId, prefix: SimpleCmd, suffix: SimpleCmd, p: Predicate<A>, cover: set<BlockId>)
   requires cfg.successors.Keys <= cfg.blocks.Keys
   requires entry in cfg.blocks
   requires cfg.blocks[entry] == SeqSimple(prefix, suffix)
   ensures 
     var cfg' := Cfg(cfg.entry, cfg.blocks[entry := suffix], cfg.successors);
-    WpCfg(a, cfg, entry, p, cover) == WpShallowSimpleCmd(a, prefix, WpCfg(a, cfg', entry, p, cover))
+    IsAcyclic(cfg.successors, entry, cover) ==> WpCfg(a, cfg, entry, p, cover) == WpShallowSimpleCmd(a, prefix, WpCfg(a, cfg', entry, p, cover))
+  {
+    if IsAcyclic(cfg.successors, entry, cover) {
+      var cfg' := Cfg(cfg.entry, cfg.blocks[entry := suffix], cfg.successors);
+      var successors := if entry in cfg.successors.Keys then cfg.successors[entry] else [];
+
+      var block := cfg.blocks[entry];
+      if successors == [] {
+        calc {
+          WpCfg(a, cfg, entry, p, cover);
+          WpShallowSimpleCmd(a, SeqSimple(prefix, suffix), p);
+          WpShallowSimpleCmd(a, prefix, WpShallowSimpleCmd(a, suffix, p));
+          WpShallowSimpleCmd(a, prefix, WpCfg(a, cfg', entry, p, cover));
+        }
+      } else {
+        calc {
+          WpCfg(a, cfg, entry, p, cover);
+          WpShallowSimpleCmd(a, SeqSimple(prefix, suffix), WpCfgConjunction(a, cfg, successors, p, cover - {entry}));
+          { assume false; }
+          WpShallowSimpleCmd(a, SeqSimple(prefix, suffix), WpCfgConjunction(a, cfg', successors, p, cover - {entry}));
+          WpShallowSimpleCmd(a, prefix, WpShallowSimpleCmd(a, suffix, WpCfgConjunction(a, cfg', successors, p, cover - {entry})));
+          WpShallowSimpleCmd(a, prefix, WpCfg(a, cfg', entry, p, cover));
+        }
+      }
+    }
+  }
   
 }
